dist/gcc-compatible/Hacl_Hash_Blake2s.c
@@ -670,8 +670,9 @@ void Hacl_Hash_Blake2s_finish(uint32_t nn, uint8_t *output, uint32_t *hash)
 /**
   State allocation function when there is no key
 */
-Hacl_Hash_Blake2s_state_t *Hacl_Hash_Blake2s_malloc(void)
+Hacl_Hash_Blake2s_state_t *Hacl_Hash_Blake2s_malloc(uint8_t *key)
 {
+  KRML_MAYBE_UNUSED_VAR(key);
   uint8_t *buf = (uint8_t *)KRML_HOST_CALLOC(64U, sizeof (uint8_t));
   uint32_t *wv = (uint32_t *)KRML_HOST_CALLOC(16U, sizeof (uint32_t));
   uint32_t *b = (uint32_t *)KRML_HOST_CALLOC(16U, sizeof (uint32_t));
@@ -688,8 +689,9 @@ Hacl_Hash_Blake2s_state_t *Hacl_Hash_Blake2s_malloc(void)
 /**
   Re-initialization function when there is no key
 */
-void Hacl_Hash_Blake2s_reset(Hacl_Hash_Blake2s_state_t *state)
+void Hacl_Hash_Blake2s_reset(Hacl_Hash_Blake2s_state_t *state, uint8_t *key)
 {
+  KRML_MAYBE_UNUSED_VAR(key);
   Hacl_Hash_Blake2s_state_t scrut = *state;
   uint8_t *buf = scrut.buf;
   Hacl_Hash_Blake2s_block_state_t block_state = scrut.block_state;
@@ -700,7 +702,7 @@ void Hacl_Hash_Blake2s_reset(Hacl_Hash_Blake2s_state_t *state)
 }
 
 /**
-  Update function when there is no key; 0 = success, 1 = max length exceeded
+  Update function when there is no key; 0ul = success, 1 = max length exceeded
 */
 Hacl_Streaming_Types_error_code
 Hacl_Hash_Blake2s_update(Hacl_Hash_Blake2s_state_t *state, uint8_t *chunk, uint32_t chunk_len)
@@ -958,7 +960,7 @@ Write the BLAKE2s digest of message `input` using key `key` into `output`.
 @param input Pointer to `input_len` bytes of memory where the input message is read from.
 @param input_len Length of the input message.
 @param key Pointer to `key_len` bytes of memory where the key is read from.
-@param key_len Length of the key. Can be 0.
+@param key_len Length of the key. Can be 0ul.
 */
 void
 Hacl_Hash_Blake2s_hash_with_key(
