code/streaming/Hacl.Streaming.Blake2b_256.fst
@@ -18,32 +18,32 @@ let blake2b_256 kk =
 
 /// Type abbreviations
 let block_state_t = Common.s Spec.Blake2B Core.M256
-let state_t = F.state_s (blake2b_256 0) () (Common.s Spec.Blake2B Core.M256) (Common.empty_key Spec.Blake2B)
+let state_t = F.state_s (blake2b_256 0ul) () (Common.s Spec.Blake2B Core.M256) (Common.empty_key Spec.Blake2B)
 
 /// No key
 inline_for_extraction noextract
 let alloca =
-  F.alloca (blake2b_256 0) () (Common.s Spec.Blake2B Core.M256) (Common.empty_key Spec.Blake2B)
+  F.alloca (blake2b_256 0ul) () (Common.s Spec.Blake2B Core.M256) (Common.empty_key Spec.Blake2B)
 
 [@ (Comment "  State allocation function when there is no key")]
 let malloc =
-  F.malloc (blake2b_256 0) () (Common.s Spec.Blake2B Core.M256) (Common.empty_key Spec.Blake2B)
+  F.malloc (blake2b_256 0ul) () (Common.s Spec.Blake2B Core.M256) (Common.empty_key Spec.Blake2B)
 
 [@ (Comment "  Re-initialization function when there is no key")]
 let reset =
-  F.reset (blake2b_256 0) () (Common.s Spec.Blake2B Core.M256) (Common.empty_key Spec.Blake2B)
+  F.reset (blake2b_256 0ul) () (Common.s Spec.Blake2B Core.M256) (Common.empty_key Spec.Blake2B)
 
-[@ (Comment "  Update function when there is no key; 0 = success, 1 = max length exceeded")]
+[@ (Comment "  Update function when there is no key; 0ul = success, 1 = max length exceeded")]
 let update =
-  F.update (blake2b_256 0) (G.hide ()) (Common.s Spec.Blake2B Core.M256) (Common.empty_key Spec.Blake2B)
+  F.update (blake2b_256 0ul) (G.hide ()) (Common.s Spec.Blake2B Core.M256) (Common.empty_key Spec.Blake2B)
 
 [@ (Comment "  Finish function when there is no key")]
 let digest =
-  F.digest (blake2b_256 0) () (Common.s Spec.Blake2B Core.M256) (Common.empty_key Spec.Blake2B)
+  F.digest (blake2b_256 0ul) () (Common.s Spec.Blake2B Core.M256) (Common.empty_key Spec.Blake2B)
 
 [@ (Comment "  Free state function when there is no key")]
 let free =
-  F.free (blake2b_256 0) (G.hide ()) (Common.s Spec.Blake2B Core.M256) (Common.empty_key Spec.Blake2B)
+  F.free (blake2b_256 0ul) (G.hide ()) (Common.s Spec.Blake2B Core.M256) (Common.empty_key Spec.Blake2B)
 
 (* The one-shot hash *)
 [@@ Comment "Write the BLAKE2b digest of message `input` using key `key` into `output`.
@@ -53,6 +53,6 @@ let free =
 @param input Pointer to `input_len` bytes of memory where the input message is read from.
 @param input_len Length of the input message.
 @param key Pointer to `key_len` bytes of memory where the key is read from.
-@param key_len Length of the key. Can be 0."]
+@param key_len Length of the key. Can be 0ul."]
 let hash_with_key : Impl.blake2_st Spec.Blake2B Core.M256 =
   Impl.blake2 #Spec.Blake2B #Core.M256 Blake2b256.init Blake2b256.update Blake2b256.finish
